imp/README.md
@@ -2,4 +2,4 @@
 
 Simple imperative programming
 
-Mostly plagiarized from [David Christiansen](git@github.com:david-christiansen/ssft24.git)
+Mostly plagiarized from [David Christiansen](https://github.com/david-christiansen/ssft24), removing bits and adding strings and arrays
